# 2.3 Homework

2024.09.28

## Exercise 1 : Evaluate the limit, if it exists.

(1) $\ \lim \limits_{x \to -2}(3x-7)$

$\ \Rightarrow 3\lim \limits_{x \to -2}x-\lim \limits_{x \to -2}7 = -6-7 = -13$

(2) $\ \lim \limits_{t \to 4} \frac{t^2-2t-8}{t-4}$

$\ \Rightarrow \lim \limits_{t \to 4} \frac{(t-4)(t+2)}{t-4} = \lim \limits_{t \to 4} t+2 = 6$

(3) $\ \lim \limits_{x \to 2} \frac{x^2+5x+4}{x-2}$

$\ \Rightarrow \lim \limits_{x \to 2} \frac{(x+1)(x+4)}{x-2}$

$\ \Rightarrow \lim \limits_{x \to 2^-}(x+1)(x+4) = \lim \limits_{x \to 2^+}(x+1)(x+4)$

$\ \Rightarrow \lim \limits_{x \to 2^-}(x-2) \neq \lim \limits_{x \to 2^+}(x-2)$

$\ \Rightarrow \lim \limits_{x \to 2^-} \frac{(x+1)(x+4)}{x-2} \neq \lim \limits_{x \to 2^+} \frac{(x+1)(x+4)}{x-2}$

$\ \Rightarrow \lim \limits_{x \to 2} \frac{(x+1)(x+4)}{x-2}$ not exists.

(4) $\ \lim \limits_{x \to 2} \frac{x^2-x-6}{3x^2+5x-2}$

$\ \Rightarrow \lim \limits_{x \to 2} \frac{(x+2)(x-3)}{(3x-1)(x+2)} = \lim \limits_{x \to 2} \frac{x-3}{3x+1} = -\frac{1}{7}$

(5) $\ \lim \limits_{t \to 3} \frac{t^3-27}{t^2-9}$

tips : $\ a^3-b^3 = (a-b)(a^2+ab+b^2)$

$\ \Rightarrow \lim \limits_{t \to 3} \frac{(t-3)(t^2+3t+9)}{(t+3)(t-3)} = \lim \limits_{t \to 3} \frac{t^2+3t+9}{t+3} = \frac{27}{6} = \frac{9}{2}$

(6) $\ \lim \limits_{h \to 0} \frac{(h-3)^2-9}{h}$

$\ \Rightarrow \lim \limits_{h \to 0} \frac{h^2-6h+9-9}{h} = \lim \limits_{h \to 0} \frac{h^2-6h}{h} = \lim \limits_{h \to 0} h-6 = -6$

(7) $\ \lim \limits_{h \to 0} \frac{\sqrt{9+h}-3}{h}$

$\ \Rightarrow \lim \limits_{h \to 0} \frac{\sqrt{9+h}-3}{h} \times \frac{\sqrt{9+h}+3}{\sqrt{9+h}+3} = \lim \limits_{h \to 0} \frac{9+h-9}{h\sqrt{9+h}+3} = \frac{1}{6}$

(8) $\ \lim \limits_{x \to 3} \frac{\frac{1}{x}-\frac{1}{3}}{x-3}$

$\ \Rightarrow \lim \limits_{x \to 3} \frac{\frac{1}{x}-\frac{1}{3}}{x-3} = \lim \limits_{x \to 3} \frac{\frac{1}{x}}{x-3}-\frac{\frac{1}{3}}{x-3} = \lim \limits_{x \to 3} x^2-3x-3x+9 = 0$

(9) $\ \lim \limits_{t \to 0} \frac{\sqrt{1+t}-\sqrt{1-t}}{t}$

$\ \Rightarrow \lim \limits_{t \to 0} \frac{\sqrt{1+t}-\sqrt{1-t}}{t} \times\frac{\sqrt{1+t}+\sqrt{1-t}}{\sqrt{1+t}+\sqrt{1-t}} = \lim \limits_{t \to 0} \frac{1+t-(1-t)}{t(\sqrt{1+t}+\sqrt{1-t})} = \lim \limits_{t \to 0} \frac{2t}{t(\sqrt{1+t}+\sqrt{1-t})} = \lim \limits_{t \to 0} \frac{2}{\sqrt{1+t}+\sqrt{1-t}} = 1?$

(10) $\ \lim \limits_{x \to 16} \frac{4-\sqrt{x}}{16x-x^2}$

$\ \Rightarrow \lim \limits_{x \to 16} \frac{4-\sqrt{x}}{x(16-x)} \times\frac{4+\sqrt{x}}{4+\sqrt{x}} = \lim \limits_{x \to 16} \frac{16-x}{x(16-x)(4+\sqrt{x})} = \lim \limits_{x \to 16} \frac{1}{x(4+\sqrt{x})} = \frac{1}{128}$

(11) $\ \lim \limits_{t \to 0} (\frac{1}{t\sqrt{1+t}} - \frac{1}{t})$

$\ \Rightarrow \lim \limits_{t \to 0} \frac{1}{t}(\frac{\sqrt{1-t}}{1-t} - \frac{1-t}{1-t}) = \lim \limits_{t \to 0} \frac{t+\sqrt{1-t}-1}{t(1-t)} = \lim \limits_{t \to 0} \frac{1}{1-t} + \lim \limits_{t \to 0} \frac{\sqrt{1-t}-1}{t(1-t)} = 1 + \lim \limits_{t \to 0} \frac{(\sqrt{1-t}-1)(\sqrt{1-t}+1)}{t(1-t)(\sqrt{1-t}+1)} = 1 + \lim \limits_{t \to 0} -\frac{1}{(1-t)(1+\sqrt{1-t})} = 1-\frac{1}{2} = \frac{1}{2}$

(12) $\ \lim \limits_{h \to 0} \frac{(x+h)^3-x^3}{h}$

$\ \Rightarrow \lim \limits_{h \to 0} \frac{x^3+3x^2h+3xh^2+h^3-x^3}{h} = \lim \limits_{h \to 0} {3x^2+3xh+h^2} = 3x^2$

## Exercuse 2 : Use the Squeeze theorem to prove that $\ \lim \limits_{x \to 0^+} \sqrt{x}e^{sin(\pi/x)}$

$\ \Rightarrow -1 \leq sin(\pi/x) \leq 1 \rightarrow \sqrt{x}e^{-1} \leq \sqrt{x}e^{sin(\pi/x)} \leq \sqrt{x}e^{1}$

$\ \because \lim \limits_{x \to 0^+} \sqrt{x}e^{-1} = 0, \lim \limits_{x \to 0^+} \sqrt{x}e^{1} = 0$

$\ \therefore \lim \limits_{x \to 0^+} \sqrt{x}e^{sin(\pi/x)} = 0$

## Exercise 3 : Find the value a such that $$\ \lim \limits_{x \to -2} \frac{3x^2+ax+a+3}{x^2+x-2}$$ exists. Then find the value of the limit.

$\ \Rightarrow \lim \limits_{x \to -2} \frac{3x^2+ax+a+3}{(x+2)(x-1)}$

$\ \rightarrow (x+2)(3x+\frac{a+3}{2}) = 3x^2+6x+(a-6)x+a+3 \rightarrow 2a-12 = a-3 \rightarrow a = 15$

$\ \Rightarrow \lim \limits_{x \to -2} \frac{(x+2)(x+9)}{(x+2)(x-1)} = -\frac{7}{3}$
