# 2.5 Limits at infinity; Horizontal Asymptoes

2024.10.09

$\ \lim \limits_{x\to\infty} \frac{x^2-1}{x^2+1} = 1$

## Def of Limit at infinity

Let $\ f$ be a function defined on $ \left\{ x|x > a \right\}$

then $\ \lim \limits_{x\to\infty} f(x) = L$ means that the value of $\ f(x)$ can be made arbitrarily close to $\ L$ by requiring $\ x$ to be sufficiertly large.

*arbitrarily 任意地 *requiring 要求 *sufficiertly 足夠地

## Def

The line $\ y = L$ is called a horizontal asymptote of the curve $\ y=f(x)$ if either $\ \lim \limits_{x\to\infty} f(x)= L$ or $\ \lim \limits_{x\to-\infty} = L$

## e.g.1 Find $\ \lim \limits_{x\to\infty} \tan^{-1}x$ and $\ \lim \limits_{x\to-\infty} \tan^{-1}x$

$\ \lim \limits_{x\to\infty} \tan^{-1}x = \frac{\pi}{2}$

$\ \lim \limits_{x\to-\infty} \tan^{-1}x = -\frac{\pi}{2}$

## e.g.2 Find $\ \lim \limits_{x\to\infty} \frac{1}{x}$ and $\ \lim \limits_{x\to-\infty} \frac{1}{x}$

|$\ x$|1000|100000|10^8|
|-|-|-|-|
|$\ \frac{1}{x}$|0.001|0.00001|0.00000001|

$\ \lim \limits_{x\to\infty} \frac{1}{x} = 0$

$\ \lim \limits_{x\to-\infty} \frac{1}{x} = 0$

## THM

If $\ r > 0$ is a rational number s.t. $\ x^r$ is defined, then 
$\ \lim \limits_{x\to\infty} \frac{1}{x^r} = 0$, $\ \lim \limits_{x\to-\infty} \frac{1}{x^r} = 0$

## e.g.3 Evaluate the limit $$\ \lim \limits_{x\to-\infty} \frac{3x^2 - x -2}{5x^2+4x+1}$$

$\ \lim \limits_{x\to\infty} \frac{3x^2 - x -2}{5x^2+4x+1} = \lim \limits_{x\to\infty} \frac{3 - \frac{1}{x} -\frac{2}{x^2}}{5+\frac{4}{x}+\frac{1}{x^2}}$

$\ \Rightarrow \frac{\lim \limits_{x\to\infty} (3 - \frac{1}{x} -\frac{2}{x^2})}{\lim \limits_{x\to\infty} (5+\frac{4}{x}+\frac{1}{x^2})} = \frac{\lim \limits_{x\to\infty} 3 - \lim \limits_{x\to\infty}\frac{1}{x} -\lim \limits_{x\to\infty}\frac{2}{x^2}}{\lim \limits_{x\to\infty} 5+\lim \limits_{x\to\infty}\frac{4}{x}+\lim \limits_{x\to\infty}\frac{1}{x^2}}$

$\ \Rightarrow \frac{3-0-0}{5+0+0} = \frac{3}{5}$

## e.g.4 Find the horizontal asymptotes of the function $$\ f(x) = \frac{\sqrt{2x^2 + 1}}{3x-5}$$

tip $\ \sqrt{x^2} = |x| = \begin{cases}
    x, x \geq 0\\
    -x, x < 0
\end{cases}$

$\ \lim \limits_{x\to\infty} \frac{\sqrt{2x^2 + 1}}{3x-5} = \lim \limits_{x\to\infty} \frac{\frac{\sqrt{2x^2 + 1}}{x}}{\frac{3x-5}{x}} = \lim \limits_{x\to\infty} \frac{\sqrt{\frac{2x^2 + 1}{x^2}}}{3-\frac{5}{x}}$

$\ = \lim \limits_{x\to\infty} \frac{\sqrt{2 + \frac{1}{x^2}}}{3-\frac{5}{x}} = \frac{\sqrt{2 + \lim \limits_{x\to\infty}\frac{1}{x^2}}}{3-5\lim \limits_{x\to\infty}\frac{1}{x}} = \frac{\sqrt{2}}{3}$

$\ \Rightarrow y = \frac{\sqrt{2}}{3}$ is a horizontal asymptote of $\ f(x)$

$\ \lim \limits_{x\to-\infty} \frac{\sqrt{2x^2 + 1}}{3x-5} = \lim \limits_{x\to-\infty} \frac{\frac{\sqrt{2x^2 + 1}}{x}}{\frac{3x-5}{x}} = \lim \limits_{x\to-\infty} \frac{\frac{\sqrt{2x^2 + 1}}{-\sqrt{x^2}}}{\frac{3x-5}{x}} = -\frac{\sqrt{2}}{3}$

$\ \Rightarrow y = -\frac{\sqrt{2}}{3}$ is also a horizontal asymptote of $\ f(x)$

## e.g.5 Compute $\ \lim \limits_{x\to-\infty} \sqrt{x^2+1}-x$

$\ \lim \limits_{x\to-\infty} \sqrt{x^2+1}-x \times \frac{\sqrt{x^2+x}}{\sqrt{x^2+x}} = \lim \limits_{x\to-\infty} \frac{1}{\sqrt{x^2+x}} = 0$