# Exercise: Differentiate

1. $g(t) = 5t + 4t^2$

    $\ \Rightarrow 8t+5$

2. $g(x) = \frac{7}{4}x^2 - 3x + 12$

    $\ \Rightarrow \frac{7}{2}x - 3$

3. $F(t) = t^3 + e^3$

    $\ \Rightarrow 3t^2$

4. $r(z) = z^{-5} - z^{\frac{1}{2}}$

    $\ \Rightarrow -5z^{-6} - \frac{1}{2}z^{-\frac{1}{2}}$

5. $V(t) = t^{-\frac{3}{5}} + t^4$

    $\ \Rightarrow -\frac{3}{5}t^{-\frac{8}{5}} + 4t^3$

6. $r(t) = \frac{a}{t^2} + \frac{b}{t^4} = at^{-2}+bt^{-4}$

    $\ \Rightarrow -2at^{-3}+-4bt^{-5}$

7. $h(w) = \sqrt{2w} - \sqrt{2} = (2w)^{0.5}+2^{0.5}$

    $\ \Rightarrow \frac{d}{dw}(2w)^{0.5} = 0.5\cdot(2w)^{-0.5}\cdot\frac{d}{dw}(2w)$

    $\ \Rightarrow (2w)^{-0.5}$

8. $W(t) = \sqrt{t} - 2e^t = t^{0.5} - 2e^t$

    $\ \Rightarrow 0.5t^{-0.5}-2e^t$

9. $S(R) = 4\pi R^2$

    $\ \Rightarrow 8\pi R$

10. $F(t) = (2t - 3)^2$

    $\ \Rightarrow \frac{d}{dw}(2t-3)^2 = 2\cdot(2t-3)\cdot\frac{d}{dw}(2t-3)$

    $\ \Rightarrow 4(2t-3)$

11. $y = \frac{\sqrt{x} + x}{x^2} = (x^{0.5}+x)\cdot x^{-2}$

    $\ f(x) = x^{0.5}+x$

    $\ f'(x) = 0.5x^{-0.5}+1$

    $\ g(x) = x^{-2}$

    $\ g'(x) = -2x^{-3}$

    $\ \Rightarrow (0.5x^{-0.5}+1)(x^{-2})+(x^{0.5}+x)(-2x^{-3})$

    $\ = -x^{-2}-1.5x^{-2.5}$

12. $G(t) = \sqrt{5t} + \frac{\sqrt{7}}{x} = (5t)^{0.5}+\sqrt{7}x^{-1}$

    $\ \Rightarrow 0.5(5t)^{-0.5}*5 = 12.5t^{-0.5}$

13. $k(r) = e^r + r e$

    $\ \Rightarrow e^r + e$

14. $G(q) = (1 + q^{-1})^2$

    $\ \Rightarrow 2\cdot(1+q^{-1})\cdot -q^{-2} = -2q^{-2}\cdot(1+q^{-1})$

15. $f(v) = \frac{\sqrt{v^3} - 2v e^v}{v} = (v^\frac{3}{2}-2ve^v)\cdot v^{-1}$

    $\ f(x) = v^\frac{3}{2}-2ve^v$

    $\ f'(x) = \frac{3}{2}v^\frac{1}{2}-(2v\cdot e^v + 2\cdot e^v) = \frac{3}{2}\sqrt{v} - e^v(2v+2)$

    $\ g(x) = v^{-1}$

    $\ g'(x) = -v^{-2}$

    $\ \Rightarrow \frac{\frac{3}{2}\sqrt{v} - e^v(2v+2)}{v} + \frac{v^\frac{3}{2}-2ve^v}{v^2}$

16. $y = e^{-x+1} + 1$

    $\ \Rightarrow e^{-x+1}\cdot-1 = -e^{-x+1}$

17. $y = (10x^2 + 7x - 2)(2 - x^2)$

    $\ \Rightarrow -2x\cdot(10x^2 + 7x - 2) + (10x+7)\cdot(2 - x^2)$

18. $y = (e^x + 2)(2e^x - 1)$

    $\ \Rightarrow 2e^x\cdot(e^x+2) + e^x\cdot(2e^x-1)$

19. $g(x) = (x + 2\sqrt{x})e^x$

    $\ \Rightarrow e^x\cdot(x+2\sqrt{x}+1+x^{-0.5})$

20. $y = \frac{e^x}{1 - e^x}$

    $\ \Rightarrow \frac{e^x}{1-2e^x}$

21. $G(u) = \frac{6u^4 - 5u}{u + 1}$

    $\ \Rightarrow \frac{24u^3-5}{u+1}+6u^4-5u$

22. $F(x) = \frac{1}{2x^3 - 6x^2 + 5} = (2x^3 - 6x^2 + 5)^{-1}$

    $\ \Rightarrow -1\cdot(2x^3 - 6x^2 + 5)\cdot(6x^2-12x)$

23. $y = \frac{\sqrt{x}}{\sqrt{x} + 1} = x^{0.5}\cdot(x^{0.5}+1)^{-1}$

    $\ f(x) = (x^{0.5}+1)^{-1}$

    $\ f'(x) = -0.5x^{-0.5}+-0.5$

    $\ \Rightarrow \frac{1}{2x+1}-\frac{1}{2}(\sqrt{x}+1)$

24. $h(w) = (w^2 + 3w)(w^{-1} - w^{-4})$

    $\ \Rightarrow (2w+3)(w^{-1} - w^{-4}) + (w^2 + 3w)(-1w^{-2} - -4w^{-5})$

25. $f(z) = (1 - e^z)(z + e^z)$

    $\ \Rightarrow -e^z(z + e^z) + (e^z+1)(1 - e^z)$

26. $W(t) = e^t(1 + te^t)$

    $\ f(t) = 1 + te^t$

    $\ f'(t) = te^t + e^t$

    $\ \Rightarrow e^t\cdot(1+te^t) + e^t\cdot(te^t + e^t)$

27. $h(r) = \frac{a e^r}{b + e^r}$

    $\ f(r) = (b+e^r)^{-1}$

    $\ f'(r) = -(b+e^r)^{-2}\cdot e^r$

    $\ \Rightarrow \frac{a e^r}{b + e^r} + (a e^r)(-(b+e^r)^{-2}\cdot e^r)$

28. $y = (z^2 + e^z)\sqrt{z}$

    $\ \Rightarrow$~~1~~

    $\ \Rightarrow \frac{z^2+e^z}{2\sqrt{z}} + \sqrt{z}(2z+e^z)$

29. $F(t) = \frac{A t}{B t^2 + C t^3}$

    $\ \Rightarrow \frac{A}{Bt^2+Ct^3} + \frac{At}{2Bt+3Ct^2}$

30. $f(x) = \frac{a x + b}{c x + d}$

    $\ \Rightarrow \frac{a}{cx+d} + \frac{ax+b}{c}$
