# 3.1 Derivatives of Polynomials and Exponential Function

2024.11.6

## Constant

$\ \frac{d}{dx}(c) = 0$

## Power rule

$\ \frac{d}{dx}(x) = 1$

$\ \frac{d}{dx}(x^n) = nx^{n-1}$

## Constant multiple

$\ \frac{d}{dx}(cf(x)) = c\frac{d}{dx}f(x)$

## Sum and difference rule

$\ \frac{d}{dx}(f(x)\pm g(x)) = \frac{d}{dx}f(x)\pm \frac{d}{dx}f(x)$

## Exponential Functions $\ f(x) = b^x$

$\ f'(x) = \lim \limits_{h \to 0} \frac{f(x+h)-f(x)}{h} = \lim \limits_{h \to 0} \frac{b^{x+h}-b^x}{h}$

$\ = \lim \limits_{h \to 0} \frac{b^x \times b^h - b^x}{h} = \lim \limits_{h \to 0} \frac{b^x \times (b^h - 1)}{h}$

$\ = b^x \times \lim \limits_{h \to 0} \frac{b^h-1}{h} = b^x \times f'(0) = f(x) \times f'(0)$

### e.g.8

* $\ \frac{d}{dx}(2^x) = 0.693 \times 2^x$

* $\ \frac{d}{dx}(3^x) = 1.099 \times 3^x$

## Def of the Number $\ e$

$\ e = \lim \limits_{x \to 0} (1+x)^{\frac{1}{x}}$

$\ \Rightarrow \lim \limits_{h \to 0} \frac{e^h-1}{h} = \lim \limits_{h \to 0} \frac{[(1+h)^\frac{1}{h}]^h-1}{h} = \lim \limits_{h \to 0} \frac{(1+h)-1}{h} = 1$

## Derivative of natural exponential function

$\ \because f'(x) = f'(0) \times f(x)$

$\ \therefore \frac{d}{dx}(e^x) = \lim \limits_{h \to 0} \frac{e^h-1}{h} \times e^x = e^x$

### e.g.9 If $\ f(x) = e^x-x$, find $\ f'$ and $\ f''$

$\ f'(x) = e^x-1$

$\ f''(x) = e^x$

### e.g.10 At what point in the curve $\ y=e^x$ is the tangent line parallel to the line $\ y=2x$

$\ f'(a) = 2 \Rightarrow e^a = 2 \Rightarrow a = ln2$

$\ f(a) = f(ln2) = e^{ln2} = 2$

$\ \Rightarrow (ln2, 2)$
