# 3.2 The Product and Quotient Rules

2024.11.6

## Product Rule

Guess $\ (fg)' = f'g'$ ?

Let $\ f(x) = x, g(x) = x^2$

$\ (fg)' = \frac{d}{dx}x^3 = 3x^2$

$\ f'g' = \frac{d}{dx}x \times \frac{d}{dx}x^2 = 1\times2x = 2x$

**Not True**

The fact: let $\ u = f(x), v = g(x)$

$\ \Delta u = f(x+\Delta x) - f(x), \Delta v = g(x+\Delta x) - g(x)$

$\ \Delta (uv) = (u+\Delta u)(v+\Delta v) - uv = v \Delta u + u \Delta v + \Delta u \Delta v$

$\ \frac{\Delta (uv)}{\Delta x} = u\frac{\Delta v}{\Delta x} + v\frac{\Delta u}{\Delta x} + \Delta u\frac{\Delta v}{\Delta x}$

$\ \frac{d}{dx}(uv) = \lim \limits_{\Delta x \to 0} \frac{\Delta (uv)}{\Delta x} = \lim \limits_{\Delta x \to 0} u\frac{\Delta v}{\Delta x} + v\frac{\Delta u}{\Delta x} + \Delta u\frac{\Delta v}{\Delta x}$

$\ = u \lim \limits_{\Delta x \to 0} \frac{\Delta v}{\Delta x} + v \lim \limits_{\Delta x \to 0} \frac{\Delta u}{\Delta x} + 0$

$\ = u \times \frac{dv}{dx} + v \times \frac{du}{dx}$

**The Product Rule :** $\ \frac{d}{dx}[f(x)g(x)] = f(x)g'(x) + f'(x)g(x)$

### e.g.1 If $\ f(x) = xe^x$, find $\ f'(x), f^{(n)}(x)$

$\ f'(x) = \frac{d}{dx}x \times e^x + x \times \frac{d}{dx} e^x = e^x + x \times e^x = (x+1)e^x$

$\ f''(x) = e^x + (x+1)e^x = (x+2)e^x$

$\ f^{(n)}(x) = (x+n)e^x$

### e.g.2 Differentiate the function $\ f(t) = \sqrt{t}(a+bt)$

**Solution 1 : Using Product rule**

$\ f'(t) = \frac{d}{dt}\sqrt{t} \times (a+bt) + \sqrt{t} \times (\frac{d}{dt}(a+bt))$

$\ = \frac{1}{2}t^{-\frac{1}{2}} + \sqrt{t} \times b$

$\ = \frac{a+bt}{2\sqrt{t}} + \frac{2bt}{2\sqrt{t}} = \frac{a+3bt}{2\sqrt{t}}$

**Solution 2 : Violence**

$\ f(t) = \sqrt{t}(a+bt) = \frac{1}{2}a(t^{-\frac{1}{2}}) + bt^{\frac{3}{2}}$

$\ f'(t) = \frac{1}{2}a\times t^{-\frac{1}{2}} + \frac{3}{2}bt^{\frac{1}{2}}$

### e.g.3 If $\ f(x) = \sqrt{x}\times g(x)$, where $\ g(4) = 2$, $\ g'(4) = 3$, find $\ f'(4)$

$\ f'(x) = \frac{d}{dx}\sqrt{x}\times g(x) + \sqrt{x}\times\frac{d}{dx}g(x)$

$\ = \frac{1}{2\sqrt{x}} \times g(x) + \sqrt{x} \times g'(x)$

$\ f'(4) = \frac{1}{4}g(4) + 2g'(4) = \frac{1}{2} + 6 = \frac{13}{2}$

## The Quotient Rule

$\ \Delta(uv) = uv(x+\Delta x) - uv(x)$

$\ = (u+\Delta u)(v+\Delta v)-uv$

$\ \Delta(\frac{u}{v}) = \frac{u+\Delta u}{v+\Delta v} - \frac{u}{v} = \frac{(u+\Delta u)\times v-u(v+\Delta v)}{(v+\Delta v)\times v}$

$\ = \frac{uv+v\Delta u-uv-u\Delta v}{(v+\Delta v)\times v} = \frac{v\Delta u-u\Delta v}{(v_\Delta v)\times v}$

$\ \frac{d}{dx}(\frac{u}{v}) = \lim \limits_{\Delta x\to 0} \frac{\Delta(\frac{u}{v})}{\Delta x} = \lim \limits_{\Delta x\to 0} \frac{v\times \frac{\Delta u}{\Delta x} - u\times \frac{\Delta v}{\Delta x}}{(v+\Delta v) \times v} = \frac{v\times u'-u\times v'}{v^2}$

**Quotient Rule**

$\ \frac{d}{dx}[\frac{f(x)}{g(x)}] = \frac{g(x)\times \frac{d}{dx}f(x)-f(x)\times \frac{d}{dx}g(x)}{[g(x)]^2}$

$\ (\frac{f}{g})' = \frac{gf'-fg'}{g^2}$

### e.g.4 Let $\ y = \frac{x^2+x-2}{x^3+6}$, Find $\ y'$

$\ y' = \frac{\frac{d}{dx}(x^2+x-2)\times(x^3+6) - (x^2+x-2)\times \frac{d}{dx}(x^3+6)}{(x^3+6)^2}$

$\ = \frac{(2x+1)(x^3+6)-(x^2+x-2)\times 3x^2}{(x^3+6)^2}$

$\ = \frac{-x^4-2x^3+6x^2+12x+6}{(x^3+6)^2}$

### e.g.5 Find an equation of the tangent line to the cyrve $\ y = \frac{e^x}{1+x^2}$ at the point $\ (1, \frac{e}{2})$

$\ \frac{dy}{dx} = \frac{\frac{d}{dx}e^x\times (1+x^2) - e^x\times \frac{d}{dx}(1+x^2)}{(1+x^2)^2}$

$\ = \frac{e^x(1+x^2) - e^x\times 2x}{(1+x^2)^2} = \frac{e^x(x-1)^2}{(1+x^2)^2}$

$\ \frac{dy}{dx} | _{x=1} = 0 \Rightarrow$ The equation of the tangent line : $\ y = \frac{e}{2}$

## Differentiation Formulas

* $\ \frac{d}{dx}(c) = 0$
* $\ \frac{d}{dx}(x^n) = n\times x^{n-1}$
* $\ \frac{d}{dx}(e^x) = e^x$
* $\ (cf)' = cf'$
* $\ (f\pm g)' = f'\pm g'$
* $\ (fg)' = f'g+fg'$
* $\ (\frac{f}{g})' = \frac{f'g-fg'}{g^2}$