# 3.4 The Chain Rule

2024.11.13

## The Chain Rule

$\ F = fã€‚g \Rightarrow F(x) = f(g(x))$

$\ F'(x) = f'(g(x)) \cdot g'(x)$

$\ F = f(u), u = g(x)$

$\ \frac{dF}{dx} = \frac{dF}{du} \cdot \frac{du}{dx}$

### e.g.1 Find $\ F'(x)$ if $\ F(x) = \sqrt{x^2+1}$

$\ F(x) = f(g(x))$

$\ F'(x) = f'(g(x)) \cdot g'(x)$

$\ g(x) = x^2 + 1$

$\ f(u) = \sqrt{u}$

$\ \Rightarrow F(x) = f(u), u = g(x)$

$\ \frac{d}{dx}F(x) = \frac{d}{dx}f(u) = \frac{d}{du}f(u)\cdot \frac{du}{dx}$

$\ f'(u) = \frac{1}{2}\cdot u^{-\frac{1}{2}}, g'(x) = 2x$

$\ F'(x) = \frac{1}{2\sqrt{u}} \cdot 2x = \frac{2x}{2\sqrt{x^2+1}}$

### e.g.2 Differentiate (a) $\ y=\sin x^2$ (b) $\ y = \sin^2 x$

(a) $\ y' = \cos x^2 \cdot 2x = 2x\cos x^2$

(b) $\ y' = 2\sin x\cos x$

### e.g.3 Differentiate $\ y - (x^3-1)^{100}$

$\ y' = 100 \cdot (x^3-1)^{99} \cdot 3x^2 = 300x^2(x^3-1)^{99}$

### e.g.4 Find $\ f'(x)$ if $\ f(x) = \frac{1}{^3\sqrt{x^2+x+1}}$

$\ f(x) = (x^2+x+1)^{-\frac{1}{3}}$

$\ f'(x) = -\frac{1}{3}(x^2+x+1)^{-\frac{4}{3}}\cdot(2x+1)$

### e.g.5 Find the derivative of the function $\ g(t) = (\frac{t-2}{2t+1})^9$

$\ g'(t) = 9(\frac{t-2}{2t+1})^8 \cdot \frac{d}{dt} \frac{t-2}{2t+1} = 9(\frac{t-2}{2t+1})^8 \cdot \frac{(2t+1)-2(t-2)}{(2t+1)^2}$

$\ g'(t) = \frac{9(t-2)^8}{(2t+1)^8} \cdot \frac{5}{(2t+1)^2} = \frac{45(t-2)^8}{(2t+1)^{10}}$

### e.g.6 Differentiate $\ y = (2x+1)^5\cdot(x^3-x+1)^4$

$\ y' = \frac{d}{dx}[(2x+1)^5](x^3-x+1)^4+(2x+1)^5\frac{d}{dx}[(x^3-x+1)^4]$

$\ = 5(2x+1)^4\cdot\frac{d}{dx}(2x+1)\cdot(x^3-x+1)^4 + (2x+1)^5\cdot4(x^3-x+1)^3\cdot\frac{d}{dx}(x^3-x+1)$

$\ = 10(2x+1)^4\cdot(x^3-x+1)^4+(12x^2-4)(2x+1)^5\cdot(x^3-x+1)^3$

$\ = 2(2x+1)^4(x^3-x+1)^3(17x^3+6x^2-9x+3)$

### e.g.7 Differentiate $\ y = e^{\sin x}$

$\ y' = e^{\sin x} \cdot \frac{d}{dx}(\sin x)$

$\ = e^{\sin x} \cdot \cos x$

### e.g.8 If $\ f(x) = \sin(\cos(\tan x))$, find $\ f'(x)$

$\ f'(x) = \cos(\cos(\tan x)) \cdot -\sin(\tan x) \cdot \sec x$

### e.g.9 Differentiate $\ y = e^{\cos 3x}$

$\ y' = e^{\cos 3x} \cdot -\sin3x \cdot 3 = -3 e^{\cos 3x} \cdot \sin3x$

## Derivatives of General Exponential functions

$\ y = b^x, (b>0)$

$\ b^x = (e^{\ln b})^x = e^{(\ln b)x}$

$\ b' = e^{(\ln b)x} \cdot \frac{d}{dx}((\ln b)x) = b^x\cdot\ln b$

### e.g.10 Find the derivative of each of the functions.

(a) $\ g(x) = 2^x$

$\ 2^x \cdot \ln 2$

(b) $\ h(x) = 5^{x^2}$

$\ 5^{x^2} \cdot \ln5 \cdot 2x$