# 3.5 Implicit Differentiation

2024.11.20

---

$\ x^2+y^2=25$

$\ y = \pm\sqrt{25-x^2}$

$\ \Rightarrow f(x) = \sqrt{25-x^2}$
$\ \Rightarrow g(x) = -\sqrt{25-x^2}$

## Implictit Differentiation

### e.g.1 If $\ x^2+y^2 = 25$, find $\ \frac{dy}{dx}$

Then find an equation of the tangent line to the circle at point (3, 4).

$\ \frac{d}{dx}x^2+\frac{d}{dx}y^2 = \frac{d}{dx}25 \Rightarrow 2x + 2y\frac{dy}{dx} = 0$

$\ \frac{dy}{dx} = -\frac{x}{y}$

when $\ x = 3, y=4 \Rightarrow \frac{dy}{dx} = -\frac{3}{4}$

### e.g.2 Find $\ y'$ if $\ x^3 + y^3 = 6xy$ and the tangent at the point (3, 3)

$\ 3x^2 + 3y^2\cdot\frac{dy}{dx} = 6y + 6x\cdot\frac{dy}{dx}$

$\ \frac{dy}{dx}(3y^2-6x) = 6y-3x^2 \Rightarrow \frac{dy}{dx} = \frac{6y-3x^2}{3y^2-6x}$

when $\ x = 3, y = 3 \Rightarrow \frac{dy}{dx} = \frac{-9}{9} = -1$

tangent : $\ y-3 = -(x-3)$

### e.g.3 Find $\ y'$ of $\ sin(x+y)=y^2\cos x$

$\ \rightarrow \frac{d}{dx}(\sin(x+y)) = \frac{d}{dx}(y^2\cos x)$

$\ \rightarrow \frac{d}{d(x+y)}(\sin(x+y))\cdot\frac{d(x+y)}{dx} = \frac{d}{dx}(y^2)\cos x+y^2\cdot \frac{d}{dx}\cos x$

$\ \cos(x+y)\cdot(1+y') = 2y\cdot y'\cdot\cos x+y^2\cdot (-\sin x)$

$\ cos(x+y)+y'\cdot\cos(x+y) = y'\cdot2y\cos^x-y^2\sin x$

$\ y'\cos(x+y)-y'\cdot 2y\cos x = -y^2\sin x-\cos(x+y)$

$\ y'[\cos(x+y)-\cdot 2y\cos x] = -y^2\sin x-\cos(x+y)$

$\ y' = \frac{-y^2\sin x-\cos(x+y)}{\cos(x+y)-\cdot 2y\cos x}$

### e.g.4 Find $\ y''$ if x^4+y^4 = 16

$\ \frac{d}{dx}x^4+\frac{d}{dx}y^4 = \frac{d}{dx}\cdot 16$

$\ \rightarrow 4x^3+4y^3\cdot y'= 0 \Rightarrow y'= -\frac{x^3}{y^3}$

$\ \rightarrow 12x^3+\frac{d}{dx}(4y^3)\cdot y'+4y^3\cdot\frac{d}{dx}\cdot y'= 0$

$\ \rightarrow 12x^3+12y^2 \cdot (y')^2+4y^3y''= 0$

$\ \rightarrow 4y^3y''= -12x^3-12y^2 \cdot \frac{x^6}{y^6}$

$\ \rightarrow 4y^3\cdot y'' = \frac{-12(x^2y^4+x^6)}{y^4} \Rightarrow y'' = \frac{-3(x^2y^4+x^6)}{y^7}$
