# Derivatives of logatithmic

2024.12.10

$\ y = log_ax\Rightarrow a^y = x$

$\ (e^x)' = e^x$

$\ 2^x = (e^{\ln2})^x = e^{x\cdot\ln2}$

$\ (2^x)' = (e^{x\cdot\ln2})' = e^{x\cdot\ln2}\cdot\ln2 = 2^x\cdot\ln2$

$\ \Rightarrow a^y\cdot\ln a\cdot y' = 1$

$\ y' = \frac{1}{a^y\cdot\ln a} = \frac{1}{x\cdot\ln a}$

$\ \frac{d}{dx}(\log_ax) = \frac{1}{x\cdot\ln a}$

$\ \frac{d}{dx}(\ln x) = \frac{1}{x}$

## Result

$\ \frac{d}{dx}(\log_ax) = \frac{1}{x\cdot\ln a}$

$\ \frac{d}{dx}(\ln x) = \frac{1}{x}$

### e.g.1 Differentiate $\ y = \ln(x^3+1)$

let $\ u = x^3+1$

$\ \frac{d}{dx} = \frac{dy}{du} \cdot \frac{du}{dx} = \frac{1}{u}\cdot3x^2 = \frac{3x^2}{x^3+1}$

### e.g.2 Find $\ \frac{d}{dx}(\ln(\sin{x}))$

$\ \frac{d}{dx}(\ln(\sin x)) = \frac{1}{\sin x}\cdot \frac{d}{dx}\sin{x} = \frac{\cos x}{\sin x}$

### e.g.3 Differentiate $\ f(x) = \sqrt{\ln x}$

$\ f'(x) = \frac{1}{2}\cdot(\ln x)^{-\frac{1}{2}}\cdot(\ln x)' = \frac{1}{2\sqrt{\ln x}}\cdot\frac{1}{x} = \frac{1}{2x\sqrt{\ln x}}$

### e.g.4 Differentiate $\ f(x) = \log_{10}(2+\sin x)$

*$\ (\log_ax)' = \frac{1}{x\cdot\ln a}$

$\ f'(x) = \frac{1}{(2+\sin x)\cdot\ln 10} \cdot \cos x = \frac{\cos x}{(2+\sin x)\cdot\ln 10}$

### e.g.5 Find $\ \frac{d}{dx} \ln\frac{x+1}{\sqrt{x-2}}$

$\ \ln\frac{x+1}{\sqrt{x-2}} = \ln(x+1)-\ln(x-2)^\frac{1}{2} = \ln(x+1)-\frac{1}{2}\ln(x-2)$

$\ \frac{d}{dx} \ln\frac{x+1}{\sqrt{x-2}} = \frac{d}{dx}\ln(x+1)-\frac{1}{2}\cdot\frac{d}{dx}\ln(x-2) = \frac{1}{x+1}-\frac{1}{2(x-2)}$

### e.g.6 Find $\ f'(x)$ if $\ f(x) = \ln|x|$

$\ f(x) = \begin{cases} \ln x, x>0 \\ \ln (-x), x<0 \\ DNE, x = 0\end{cases}$

$\ f'(x) = \begin{cases} \frac{1}{x}, x>0 \\ \frac{1}{-x}\cdot-1 = \frac{1}{x}, x<0\end{cases}$

$\ f'(x) = \frac{1}{x}, x \neq 0$

### e.g.7 Differentiate $\ y = \frac{x^\frac{3}{4}\sqrt{x^2+1}}{(3x+2)^5}$

$\ \ln y = \ln \frac{x^\frac{3}{4}\sqrt{x^2+1}}{(3x+2)^5}$

$\ = \ln x^\frac{3}{4} + \ln \sqrt{x^2+1} - \ln(3x+2)^5$

$\ = \frac{3}{4} \ln x + \frac{1}{2} \ln x^2+1 - 5\ln3x+2$

Differentiate :

$\ \frac{1}{y} \cdot y' = \frac34 \cdot \frac 1x + \frac 12 \cdot \frac{x^2+1}{1} \cdot 2x - 5 \cdot \frac{1}{3x+2} \cdot 3$

$\ y' = y \times (\frac{3}{4x} + \frac{x}{x^2+1} - \frac{15}{3x+2}) = \frac{x^\frac{3}{4}\sqrt{x^2+1}}{(3x+2)^5} \cdot (\frac{3}{4x} + \frac{1}{x^2+1} - \frac{15}{3x+2})$

## Derivatives of Inverse trigonometric functions

$\ y = \sin^{-1}(x) = arcsine(x) \iff \sin{y} = x, -\frac{\pi}{2} \leq y \leq \frac{\pi}{2}$

$\ \frac{d}{dx} \sin{y} = \frac{d}{dx} x$

$\ \cos y \cdot \frac{dy}{dx} = 1 \Rightarrow \frac{dy}{dx} = \frac{1}{\cos y}$

$\ \cos y = \sqrt{1-x^2}$

$\ y' = \frac{d}{dx}(\sin^{-1}x)= \frac{1}{\sqrt{1-x^2}}$

### e.g.8 Differentiate $\ y = \cos^{-1}x$

$\ y = \cos^{-1}x \Rightarrow \cos{y} = x, 0\leq y\leq \pi$

$\ \frac{d}{dx} \cos{y} = \frac{d}{dx} x$

$\ -\sin y \cdot \frac{dy}{dx} = 1$

$\ y' = \frac{1}{-\sin y} = \frac{-1}{\sqrt{1-x^2}}$

### e.g.9 Differentiate $\ y = \tan^{-1}x$

$\ \tan{y} = x$

$\ \frac{dy}{dx} \cdot \sec^2{y} = 1 \Rightarrow y' = \frac{1}{\sec^2 y}$

$\ \tan^2 y + 1 = \sec^2 y \Rightarrow \sec^2 y = 1+x^2$

$\ y' = \frac{1}{1+x^2}$

### e.g.10 Differentiate $\ y = \frac{1}{\sin^{-1}x}$

$\ \frac{dy}{dx} = \frac{d}{dx}[\sin^{-1} x]^{-1} = -(\sin^{-1} x)^{-2} \cdot \frac{d}{dx} \sin^{-1} x$

$\ = \frac{-1}{(\sin^{-1}x)^2} \cdot \frac{1}{\sqrt{1-x^2}}$

$\ = -\frac{1}{(\sin^{-1}x)^2\cdot\sqrt{1-x^2}}$

Other way :

$\ \frac{1}{y} = \sin^{-1}x \Rightarrow \sin \frac1y = x$

$\ \frac{d}{dx} \sin \frac1y = \frac{d}{dx} x$

$\ \cos\frac1y\cdot\frac{-1}{y^2}\cdot y' = 1 \Rightarrow ...$

### e.g.11 Differentiate $\ f(x) = x \arctan\sqrt x$

$\ f'(x) = \arctan\sqrt x + x\cdot\frac{d}{dx}(\arctan\sqrt x)$

$\ = \arctan\sqrt x + x\cdot\frac{1}{1+(\sqrt x)^2}\cdot\frac{1}{2}\cdot x^{-\frac{1}{2}}$

$\ = \arctan\sqrt x + \frac{\sqrt x}{2(1+x)}$

### e.g.12 Differentiate $\ g(x) = sec^{-1}(x^2)$

$\ \sec{y} = x^2$

$\ {\cos{y}}^{-1} = x^2$

$\ \frac{d}{dx}{\cos{y}}^{-1} = \frac{d}{dx}x^2$

$\ -\cos y ^{-2} \cdot -\sin y \cdot y' = 2x$

$\ -\sin y \cdot y' = -2x \cdot (\cos y)^2$

$\ y' = \frac{2x \cdot \frac{1}{x^4}}{\frac{\sqrt{x^4-1}}{x^2}} = \frac{2}{x\sqrt{x^4-1}}$
